format-version: 1.2
ontology: hp/imports/mpath_import

[Term]
id: MPATH:0
name: pathological entity
namespace: mouse_pathology.ontology
def: "Pathological structure or process" [Pathbase: Curation]

[Term]
id: MPATH:1
name: cell and tissue damage
namespace: mouse_pathology.ontology
def: "The sum of morphological and functional disturbances induced by cell and tissue damage, either from intrinsic gene dysfunction or as a result of external factors." [Pathbase: Pathology Committee]
is_a: MPATH:603 ! pathological anatomical entity

[Term]
id: MPATH:105
name: circulatory disorder
namespace: mouse_pathology.ontology
def: "Lesions leading to or consequent on failure of, or atypical movement of, blood throughout the body." [Pathbase: Pathology Committee]
is_a: MPATH:603 ! pathological anatomical entity

[Term]
id: MPATH:119
name: hemorrhage and non-specified extravasation
namespace: mouse_pathology.ontology
def: "Abnormal release of whole blood or the cellular component from the circulation." [Pathbase: Curation]
is_a: MPATH:105 ! circulatory disorder

[Term]
id: MPATH:120
name: ecchymosis
namespace: mouse_pathology.ontology
def: "A red/purple patch caused by extravasation of blood into the skin. Larger than petechiae." [ISBN:0781727286]
comment: May also be used for any organ, although more generally used with respect to the skin.
is_a: MPATH:119 ! hemorrhage and non-specified extravasation

[Term]
id: MPATH:121
name: hematoma
namespace: mouse_pathology.ontology
def: "A localised deposition of clotted or partially clotted extravasated blood." [ISBN:0781727286]
synonym: "Bruise" RELATED [Pathbase: Curation]
is_a: MPATH:119 ! hemorrhage and non-specified extravasation

[Term]
id: MPATH:124
name: infarct
namespace: mouse_pathology.ontology
def: "An area of necrosis resulting from a sudden cessation of arterial or venous blood supply." [Pathbase: Pathology Committee]
is_a: MPATH:105 ! circulatory disorder

[Term]
id: MPATH:126
name: growth and differentiation defect
namespace: mouse_pathology.ontology
def: "Defects in growth (changes in proliferation or mass) and differentiation of cells tissues or organs." [Pathbase: Pathology Committee]
is_a: MPATH:603 ! pathological anatomical entity

[Term]
id: MPATH:127
name: atrophy
namespace: mouse_pathology.ontology
def: "A reduction in size of organs or tissues as a result of cell death, loss of cellularity of whatever cause, reduced cellular proliferation or decreased cellular volume." [Pathbase: Pathology Committee]
is_a: MPATH:604 ! defective growth and differentiation process

[Term]
id: MPATH:14
name: process of degenerative change
namespace: mouse_pathology.ontology
def: "A pathological process of loss or degradation of function, or structural integrity, of a tissue, organ or cell." [Pathbase: Pathology Committee]
is_a: MPATH:597 ! cell and tissue damage process
created_by: George Gkoutos

[Term]
id: MPATH:149
name: squamous hyperplasia
namespace: mouse_pathology.ontology
def: "Benign proliferation of epidermal cells with hyperkeratosis. Variable growth pattern, regular to papillary (exophytic squamous cell hyperplasia)." [Pathbase: Pathology Committee]
synonym: "epidermal hyperplasia." RELATED [Pathbase: Curation]
synonym: "squamous cell hyperplasia" RELATED [Pathbase: Curation]
is_a: MPATH:602 ! hyperplastic tissue
created_by: George Gkoutos

[Term]
id: MPATH:150
name: acanthosis
namespace: mouse_pathology.ontology
def: "Hyperplasia of the Malpighian layer (prickle cell) of the epidermis." [ISBN:0781727286]
is_a: MPATH:149 ! squamous hyperplasia
created_by: George Gkoutos

[Term]
id: MPATH:154
name: hyperkeratosis
namespace: mouse_pathology.ontology
def: "Thickening of the surface layers (stratum corneum) in the skin or other stratified squamous epithelium. Cf. ortho- and para-keratosis." [Pathbase: Pathology Committee]
synonym: "cornification" RELATED [Pathbase: Curation]
synonym: "hyperorthokeratosis" RELATED [Pathbase: Curation]
synonym: "hyperparakeratosis" RELATED [Pathbase: Curation]
is_a: MPATH:149 ! squamous hyperplasia
created_by: George Gkoutos

[Term]
id: MPATH:156
name: parakeratosis
namespace: mouse_pathology.ontology
def: "Thickening of the surface cell layer of a stratified squamous epithelium with retention of nuclei in the cells of the stratum corneum." [Pathbase: Pathology Committee]
is_a: MPATH:154 ! hyperkeratosis
created_by: George Gkoutos

[Term]
id: MPATH:160
name: metaplasia
namespace: mouse_pathology.ontology
def: "Abnormal transformation of an fully differentiated adult cell or tissue of one kind into a differentiated tissue of another kind. An adult instance of developmental transdifferentiation MPATH:85 Traditionally defined as a form of abnormal regeneration in which a type of cell different from that found normally in a given location is produced." [Pathbase: Pathology Committee]
is_a: MPATH:604 ! defective growth and differentiation process
created_by: George Gkoutos

[Term]
id: MPATH:162
name: epithelial metaplasia
namespace: mouse_pathology.ontology
def: "Metaplasia occurring within epithelia." [ISBN:0781727286]
is_a: MPATH:605 ! metaplastic tissue
created_by: George Gkoutos

[Term]
id: MPATH:164
name: gastric metaplasia
namespace: mouse_pathology.ontology
def: "Appearance of heterotopic gastric epithelium." [ISBN:0781727286]
is_a: MPATH:162 ! epithelial metaplasia
created_by: George Gkoutos

[Term]
id: MPATH:175
name: healing and repair process
namespace: mouse_pathology.ontology
def: "The process, normal or abnormal, of damage repair or wound closure." [Pathbase: Pathology Committee]
is_a: MPATH:596 ! pathological process
created_by: George Gkoutos

[Term]
id: MPATH:176
name: connective tissue replacement
namespace: mouse_pathology.ontology
def: "Replacement of connective tissue by fibro-fatty deposits and scar tissue." [Pathbase: Curation]
is_a: MPATH:175 ! healing and repair process
created_by: George Gkoutos

[Term]
id: MPATH:181
name: fibrosis
namespace: mouse_pathology.ontology
def: "Reactive formation of fibrous tissue." [Pathbase: Curation]
is_a: MPATH:176 ! connective tissue replacement
created_by: George Gkoutos

[Term]
id: MPATH:184
name: sclerosis
namespace: mouse_pathology.ontology
def: "Any pathological thickening or hardening of a tissue." [Pathbase: Curation]
synonym: "Induration" RELATED [Pathbase: Curation]
is_a: MPATH:176 ! connective tissue replacement
created_by: George Gkoutos

[Term]
id: MPATH:188
name: immunopathological process
namespace: mouse_pathology.ontology
def: "Inappropriate or aberrant activation or suppression of the immune or inflammatory response." [Pathbase: Pathology Committee]
is_a: MPATH:596 ! pathological process
created_by: George Gkoutos

[Term]
id: MPATH:194
name: immune mediated disease
namespace: mouse_pathology.ontology
def: "Tissue response to inappropriate immune/inflammatory process." [Pathbase: Curation]
is_a: MPATH:188 ! immunopathological process
created_by: George Gkoutos

[Term]
id: MPATH:195
name: arthritis
namespace: mouse_pathology.ontology
def: "Inflammation of a joint." [Pathbase: Curation]
is_a: MPATH:212 ! inflammation
created_by: George Gkoutos

[Term]
id: MPATH:196
name: dermatitis
namespace: mouse_pathology.ontology
def: "Inflammation of the skin." [Pathbase: Curation]
is_a: MPATH:212 ! inflammation
created_by: George Gkoutos

[Term]
id: MPATH:197
name: glomerulonephritis
namespace: mouse_pathology.ontology
def: "Renal disease characterised by diffuse inflammatory changes in glomeruli not in response to an infectious agent or treatment." [Pathbase: Curation]
is_a: MPATH:212 ! inflammation
created_by: George Gkoutos

[Term]
id: MPATH:198
name: immune mediated hemolytic anaemia
namespace: mouse_pathology.ontology
def: "An anemic/erythrocytopenic condition resulting from an increased rate of immune mediated erythrocyte destruction." [ISBN:0781727286]
is_a: MPATH:212 ! inflammation
created_by: George Gkoutos

[Term]
id: MPATH:2
name: cell death
namespace: mouse_pathology.ontology
def: "Complete and irreversible cessation of metabolic activity." [Pathbase: Pathology Committee]
is_a: MPATH:597 ! cell and tissue damage process
created_by: George Gkoutos

[Term]
id: MPATH:200
name: myositis
namespace: mouse_pathology.ontology
def: "Inflammation of a muscle." [Pathbase: Curation]
synonym: "Initis" RELATED [Pathbase: Curation]
is_a: MPATH:212 ! inflammation
created_by: George Gkoutos

[Term]
id: MPATH:201
name: vasculitis
namespace: mouse_pathology.ontology
def: "Inflammation of a blood vessel." [Pathbase: Pathology Committee]
synonym: "angiitis" RELATED [Pathbase: Curation]
synonym: "arteritis" RELATED [Pathbase: Curation]
synonym: "lymphangiitis" RELATED [Pathbase: Curation]
synonym: "phlebitis" RELATED [Pathbase: Curation]
is_a: MPATH:212 ! inflammation
created_by: George Gkoutos

[Term]
id: MPATH:212
name: inflammation
namespace: mouse_pathology.ontology
def: "A tissue reaction to an internal or external injury." [Pathbase: Pathology Committee]
is_a: MPATH:194 ! immune mediated disease
created_by: George Gkoutos

[Term]
id: MPATH:213
name: acute inflammation
namespace: mouse_pathology.ontology
def: "Inflammation with a recent onset, characterised histologically by primarily granulocyte infiltration, edema and hyperemia." [Pathbase: Pathology Committee]
comment: The five classical signs of inflammation: Rubor, tumor, calor, dolor, functio laesa (Galen 300BC).
is_a: MPATH:212 ! inflammation
created_by: George Gkoutos

[Term]
id: MPATH:214
name: chronic inflammation
namespace: mouse_pathology.ontology
def: "Chronic inflammatory condition characterised by infiltration of primarily lymphocytes." [Pathbase: Pathology Committee]
is_a: MPATH:212 ! inflammation
created_by: George Gkoutos

[Term]
id: MPATH:218
name: neoplasm
namespace: mouse_pathology.ontology
def: "A tumor resulting from abnormal and uncontrolled autonomous new cell growth (proliferation)that may be benign or malignant." [Pathbase: Pathology Committee]
is_a: MPATH:603 ! pathological anatomical entity
created_by: George Gkoutos

[Term]
id: MPATH:219
name: adnexal and skin appendage tumor
namespace: mouse_pathology.ontology
def: "Tumors of the skin, its constituent structures and glands including the mammary gland, apocrine and eccrine glands, hair follicles and associated structures." [Pathbase: Curation]
is_a: MPATH:218 ! neoplasm
created_by: George Gkoutos

[Term]
id: MPATH:232
name: trichoepithelioma
namespace: mouse_pathology.ontology
def: "Multiple small benign nodules derived from basal cells of hair follicles enclosing small cornified cell containing cysts. (M-8100/0)." [URL:http\://emice.nci.nih.gov/emice/mouse_models/organ_models/skin_models]
synonym: "benign" RELATED [Pathbase: Curation]
synonym: "Epithelioma adenoides cysticum" RELATED [Pathbase: Curation]
synonym: "hair follicle tumor" RELATED [Pathbase: Curation]
is_a: MPATH:575 ! basaloid follicular neoplasms

[Term]
id: MPATH:233
name: basal cell tumor
namespace: mouse_pathology.ontology
def: "Well circumscribed tumor of the basal cells of the epidermis. Rare mitotic figures, benign. (M8147/0)." [Pathbase: Pathology Committee]
synonym: "basal cell adenoma" RELATED [Pathbase: Curation]
synonym: "Benign basal cell tumor" RELATED [Pathbase: Curation]
is_a: MPATH:219 ! adnexal and skin appendage tumor
is_a: MPATH:270 ! adenoma

[Term]
id: MPATH:234
name: basal cell carcinoma
namespace: mouse_pathology.ontology
def: "Malignant neoplasm of the basal cells of the epidermis with local invasion. (M-8090/3)." [URL:http\://emice.nci.nih.gov/emice/mouse_models/organ_models/skin_models]
is_a: MPATH:549 ! carcinoma
is_a: MPATH:575 ! basaloid follicular neoplasms

[Term]
id: MPATH:235
name: blood vessel tumor
namespace: mouse_pathology.ontology
def: "Tumor of venous or arterial vessels or capillaries." [Pathbase: Pathology Committee]
is_a: MPATH:218 ! neoplasm

[Term]
id: MPATH:236
name: angiofibroma
namespace: mouse_pathology.ontology
def: ".A benign neoplasm of fibrous tissue in which there are multiple large and small dilated vascular channels ( M9160/0)." [Pathbase: Curation]
synonym: "Telangiectatic fibroma" RELATED [Pathbase: Curation]
is_a: MPATH:235 ! blood vessel tumor

[Term]
id: MPATH:238
name: hemangioblastoma
namespace: mouse_pathology.ontology
def: "A benign neoplasm frequently arising in the cerebellum composed of capillary vessel forming endothelial cells and stromal cells. (M-9161/1)." [Pathbase: Pathology Committee]
synonym: "Angioblastoma" RELATED [Pathbase: Curation]
is_a: MPATH:235 ! blood vessel tumor

[Term]
id: MPATH:240
name: hemangioma
namespace: mouse_pathology.ontology
def: "Neoplasm derived from endothelial cells. May be of capillary or cavernous type with large vascular channels. (M-9130/0 + M-9120/0 respectively)." [PMID:8569146]
synonym: "Angioendothelioma." RELATED [Pathbase: Curation]
synonym: "Hemangioendothelioma, benign" RELATED [Pathbase: Curation]
is_a: MPATH:235 ! blood vessel tumor

[Term]
id: MPATH:242
name: hemangiosarcoma
namespace: mouse_pathology.ontology
def: "Malignant neoplasm derived from pluripotential mesenchymal stem cells or endothelial cells of blood vessels. (M-9120/3)." [PMID:8569146]
synonym: "hemangioendothelioma malignant, angiosarcoma" RELATED [Pathbase: Curation]
synonym: "hemangioendothelioma malignant." RELATED [Pathbase: Curation]
synonym: "Hemangioma malignant" RELATED [Pathbase: Curation]
is_a: MPATH:235 ! blood vessel tumor
is_a: MPATH:551 ! sarcoma

[Term]
id: MPATH:243
name: central nervous system tumor
namespace: mouse_pathology.ontology
def: "Neoplasm of the neurones, glia or meninges of the CNS." [Pathbase: Curation]
is_a: MPATH:218 ! neoplasm

[Term]
id: MPATH:244
name: astrocytoma
namespace: mouse_pathology.ontology
def: "Glioma derived from astrocytes, both benign and malignant forms (M-9400/3)." [ISBN-13:9783794515530]
comment: Also see comments in Weiss, W.W, Israel, M. Cobbs, C., et al. (2002) Oncogene 21, 7453-7463.
synonym: "Astrocytic glioma" RELATED [Pathbase: Curation]
synonym: "astroglioma" RELATED [Pathbase: Curation]
is_a: MPATH:249 ! glioma

[Term]
id: MPATH:246
name: choroid plexus papilloma
namespace: mouse_pathology.ontology
def: "Benign neoplasm derived from the epithelial cells of the choroid plexus. (M-9390/0)." [ISBN-13:9783794515530]
is_a: MPATH:264 ! fibroepithelial tumor
is_a: MPATH:565 ! tumors of neurepithelial tissue

[Term]
id: MPATH:247
name: ependymoma
namespace: mouse_pathology.ontology
def: "Neoplasm derived from the ependymal cells lining the ventricles and aqueduct of the brain and the central canal of the spinal cord. Malignant or benign. (M-9391/3)." [ISBN-13:9783794515530]
comment: Also see general scheme in Weiss, W.W, Israel, M. Cobbs, C., et al. (2002) Oncogene 21, 7453-7463.
is_a: MPATH:249 ! glioma

[Term]
id: MPATH:249
name: glioma
namespace: mouse_pathology.ontology
def: "Neoplasm derived from astrocytes and oligodendrocytes. (M-9380/3, M-9440/3)." [ISBN-13:9783794515530]
comment: Also see comments in: Weiss, W.W, Israel, M. Cobbs, C., et al. (2002) Oncogene 21, 7453-7463.
is_a: MPATH:565 ! tumors of neurepithelial tissue

[Term]
id: MPATH:25
name: tissue specific degenerative process
namespace: mouse_pathology.ontology
def: "Degenerative process characteristic of a particular tissue." [Pathbase: Curation]
is_a: MPATH:14 ! process of degenerative change

[Term]
id: MPATH:250
name: medulloblastoma
namespace: mouse_pathology.ontology
def: "Neoplasm derived from the primitive neurectodermal cells of the cerebellum. (M-9470/3). May be considered by some authorities a synonym of PNET in the CNS." [ISBN-13:9783794515530]
comment: Also see Weiss, W.W, Israel, M. Cobbs, C., et al. (2002) Oncogene 21, 7453-7463.
is_a: MPATH:373 ! CNS progenitor tumor

[Term]
id: MPATH:251
name: meningioma
namespace: mouse_pathology.ontology
def: "meningioma" [ISBN-13:9783794515530]
comment: Benign or malignant neoplasm derived from the meninges. (M-9530/0).
synonym: "Sarcoma, meningeal ( sensu malignant tumor)" RELATED [Pathbase: Curation]
is_a: MPATH:566 ! tumors of the meninges

[Term]
id: MPATH:252
name: oligodendroglioma
namespace: mouse_pathology.ontology
def: "Benign or malignant neoplasm derived form oligodendrocytes (M-9450/3)." [ISBN-13:9783794515530]
comment: Also see Weiss, W.W, Israel, M. Cobbs, C., et al. (2002) Oncogene 21, 7453-7463.
synonym: "glioma oligodendritic, malignant" RELATED [Pathbase: Curation]
synonym: "Glioma, oligodendritic, benign" RELATED [Pathbase: Curation]
is_a: MPATH:249 ! glioma

[Term]
id: MPATH:254
name: complex tumor
namespace: mouse_pathology.ontology
def: "Tumors showing mutiple histological componants/differentiation." [Pathbase: Pathology Committee]
is_a: MPATH:218 ! neoplasm

[Term]
id: MPATH:261
name: nephroblastoma
namespace: mouse_pathology.ontology
def: "Embryonal tumor thought to be derived from metanephric blastema. Mono, bi or triphasic, sometimes with heterotypic differentiation. (M-8960/3)." [Pathbase: Pathology Committee]
synonym: "nephroma" RELATED [Pathbase: Curation]
is_a: MPATH:254 ! complex tumor

[Term]
id: MPATH:262
name: pulmonary blastoma
namespace: mouse_pathology.ontology
def: "A biphasic tumor containing a primitive epithelial component, that may resemble well-differentiated fetal adenocarcinoma and a primitive mesenchymal stroma, which occasionally has foci of osteosarcoma, chondrosarcoma or rhadomyosarcoma. (M-8972/3)." [Pathbase: Pathology Committee]
is_a: MPATH:254 ! complex tumor

[Term]
id: MPATH:264
name: fibroepithelial tumor
namespace: mouse_pathology.ontology
def: "Tumors with epithelial invaginations/linings and a fibrillary and fibrocytic stroma. (M-9000 - M-9030)." [Pathbase: Curation]
is_a: MPATH:218 ! neoplasm

[Term]
id: MPATH:266
name: fibroadenoma
namespace: mouse_pathology.ontology
def: "A benign neoplasm derived from glandular epithelium, in which there is a abundant stroma of proliferating fibroblasts and connective tissue. (M-9010/0)." [Pathbase: Curation]
is_a: MPATH:264 ! fibroepithelial tumor

[Term]
id: MPATH:267
name: glandular tumor
namespace: mouse_pathology.ontology
def: "Neoplasms derived from glandular epithelial cells." [Pathbase: Curation]
is_a: MPATH:218 ! neoplasm

[Term]
id: MPATH:268
name: adenocarcinoma
namespace: mouse_pathology.ontology
def: "Malignant neoplasm of epithelial cells in glandular or glandlike pattern. (M-8140/3)." [Pathbase: Curation]
is_a: MPATH:267 ! glandular tumor
is_a: MPATH:549 ! carcinoma

[Term]
id: MPATH:27
name: arthrosis
namespace: mouse_pathology.ontology
def: "Changes characterized by erosion of articular cartilage, either primary or secondary to trauma or other conditions. Not primarily an inflammatory process." [ISBN:0781727286]
synonym: "Degenerative joint disease" RELATED [Pathbase: Curation]
synonym: "osteoarthrosis" RELATED [Pathbase: Curation]
is_a: MPATH:25 ! tissue specific degenerative process

[Term]
id: MPATH:270
name: adenoma
namespace: mouse_pathology.ontology
def: "A benign epithelial neoplasm in which the tumor cells may form glands or glandlike structures. In different instances this may remain a benign tumor or progress to malignancy." [Pathbase: Pathology Committee]
is_a: MPATH:267 ! glandular tumor
is_a: MPATH:556 ! potentially cancerous lesions

[Term]
id: MPATH:271
name: adenomatous polyposis coli
namespace: mouse_pathology.ontology
def: "Spontaneous intestinal adenoma formation. Polyps increase in number, causing symptoms of chronic colitis and potentially transform into adenocarcinoma. (M-8220/0)." [Pathbase: Curation]
is_a: MPATH:267 ! glandular tumor
is_a: MPATH:556 ! potentially cancerous lesions

[Term]
id: MPATH:277
name: cystadenoma
namespace: mouse_pathology.ontology
def: "A benign neoplasm derived from glandular epithelium, in which cystic accumulations of retained secretions are formed. (M-8440/0)." [Pathbase: Pathology Committee]
is_a: MPATH:270 ! adenoma

[Term]
id: MPATH:278
name: follicular adenocarcinoma
namespace: mouse_pathology.ontology
def: "Originates in the follicular cells of thyroid follicles. Papillary, solid and follicular forms. (M- 8330/3)." [Pathbase: Curation]
synonym: "Follicular carcinoma" RELATED [Pathbase: Curation]
is_a: MPATH:268 ! adenocarcinoma

[Term]
id: MPATH:28
name: atherosclerosis
namespace: mouse_pathology.ontology
def: "Characterised by irregular lipid deposits in the wall of arteries, causing narrowing of their lumens and proceeding eventually to fibrosis and calcification." [Pathbase: Pathology Committee]
comment: Note that in mouse and rats the initial lesions are mostly in the medial layer while in human they occur in the intima.
is_a: MPATH:25 ! tissue specific degenerative process

[Term]
id: MPATH:287
name: islet cell adenoma
namespace: mouse_pathology.ontology
def: "Usually pancreatic B cell derived tumors mostly producing insulin. (M- 8150/0)." [Pathbase: Curation]
synonym: "Adenoma, endocrine pancreas" RELATED [Pathbase: Curation]
synonym: "adenomatosis" RELATED [Pathbase: Curation]
synonym: "islet (pancreatic) cell tumor benign" RELATED [Pathbase: Curation]
is_a: MPATH:270 ! adenoma

[Term]
id: MPATH:291
name: medullary carcinoma
namespace: mouse_pathology.ontology
def: "Derived from calcitonin-producing cells (thyroid). In humans a type of carcinoma composed of epithelial elements with considerable lymphoid stroma (breast). Not yet reported in mice. (M-8510/3)." [Pathbase: Pathology Committee]
synonym: "Medullary adenocarcinoma" RELATED [Pathbase: Curation]
is_a: MPATH:267 ! glandular tumor
is_a: MPATH:549 ! carcinoma

[Term]
id: MPATH:295
name: papillary adenocarcinoma
namespace: mouse_pathology.ontology
def: "A malignant neoplasm derived from a glandular epithelium, in which solid tumors show papillary structures projecting onto fibrovascular stroma. (M-8260/3)." [Pathbase: Pathology Committee]
is_a: MPATH:268 ! adenocarcinoma

[Term]
id: MPATH:298
name: papillary cystadenoma
namespace: mouse_pathology.ontology
def: "A benign neoplasm derived from glandular epithelium, in which cysts contain folds or papillary projections into the lumen. (M-8450/0)." [Pathbase: Pathology Committee]
is_a: MPATH:270 ! adenoma

[Term]
id: MPATH:299
name: pinealoma
namespace: mouse_pathology.ontology
def: "Originating from differentiated cells of the pineal parenchyma. Not to be confused with human pinealoma (syn: germinoma) non-gonadal germ cell tumors found in the pineal believed to be atypical teratomas. May be benign or malignant. If ectopic teratomas/teratocarcinomas use MP322 or MP321. (M-9360/1)." [Pathbase: Pathology Committee]
is_a: MPATH:267 ! glandular tumor

[Term]
id: MPATH:308
name: thyroid C-cell carcinoma
namespace: mouse_pathology.ontology
def: "Malignant neoplasm derived from the calcitonin producing C-cells of the thyroid gland. (M-8510/3, M-8345/3)." [Pathbase: Curation]
synonym: "Medullary carcinoma, parafollicular cell" RELATED [Pathbase: Curation]
synonym: "tumor c-cell malignant" RELATED [Pathbase: Curation]
is_a: MPATH:267 ! glandular tumor
is_a: MPATH:549 ! carcinoma

[Term]
id: MPATH:309
name: gonadal tumor
namespace: mouse_pathology.ontology
def: "Germ cell and non-germ cell tumors of the testis and ovary." [Pathbase: Pathology Committee]
is_a: MPATH:218 ! neoplasm

[Term]
id: MPATH:31
name: emphysema
namespace: mouse_pathology.ontology
def: "Abnormal accumulation of air in the interstitial connective tissue of a structure. Sensu Lung: Pulmonary emphysema; characterised by abnormal increase in the size of air (alveolar) spaces distal to the terminal bronchiole with degenerative changes in their walls and reduction in their number." [ISBN:0781727286]
is_a: MPATH:25 ! tissue specific degenerative process

[Term]
id: MPATH:310
name: germ cell tumor
namespace: mouse_pathology.ontology
def: "Neoplasms derived from germ cells. May be gonadal or extragonadal and are derived from primordial germ cells." [Pathbase: Pathology Committee]
is_a: MPATH:309 ! gonadal tumor

[Term]
id: MPATH:312
name: dysgerminoma
namespace: mouse_pathology.ontology
def: "Undifferentiated germ cell tumor of the ovary composed of solid sheets of large polygonal cells with rim of clear cytoplasm (M-9060/3)." [Pathbase: Curation]
synonym: "Seminoma (sensu male)" RELATED [Pathbase: Curation]
is_a: MPATH:310 ! germ cell tumor

[Term]
id: MPATH:315
name: gonadoblastoma
namespace: mouse_pathology.ontology
def: "Gonadal neoplasms that consist of aggregates of germ cells and sex cord elements (M-9073/1)." [Pathbase: Curation]
synonym: "Gonocytoma" RELATED [Pathbase: Curation]
is_a: MPATH:310 ! germ cell tumor

[Term]
id: MPATH:316
name: mixed germ cell tumor
namespace: mouse_pathology.ontology
def: "Malignant neoplasm of the testis/ovary including various elements of germ cell tumors (M-9085/3)." [Pathbase: Curation]
synonym: "Mixed teratoma and seminoma" RELATED [Pathbase: Curation]
is_a: MPATH:254 ! complex tumor
is_a: MPATH:310 ! germ cell tumor

[Term]
id: MPATH:317
name: seminoma
namespace: mouse_pathology.ontology
def: "Tumor derived from spermatogenic cells resembling spermatogenia or spermatocytes. NOS ( M9061/3)." [Pathbase: Curation]
synonym: "dysgerminoma" RELATED [Pathbase: Curation]
synonym: "Germinoma, malignant" RELATED [Pathbase: Curation]
synonym: "spermatoblastoma" RELATED [Pathbase: Curation]
synonym: "spermatocytoma, malignant." RELATED [Pathbase: Curation]
is_a: MPATH:310 ! germ cell tumor

[Term]
id: MPATH:321
name: teratocarcinoma
namespace: mouse_pathology.ontology
def: "Mixed germ cell neoplasm contaning elements of embryonal carcinoma and teratoma (M-9081/3)." [Pathbase: Curation]
is_a: MPATH:254 ! complex tumor
is_a: MPATH:310 ! germ cell tumor
is_a: MPATH:549 ! carcinoma

[Term]
id: MPATH:322
name: teratoma
namespace: mouse_pathology.ontology
def: "Generally benign germ cell derived tumors of male or female containing derivatives from all three germ layers with differentiation in the malignant form being poor. Malignant tumors are highly metatstatic. (M-9080/1)." [Pathbase: Pathology Committee]
is_a: MPATH:254 ! complex tumor
is_a: MPATH:310 ! germ cell tumor

[Term]
id: MPATH:323
name: gonadal somatic cell tumor
namespace: mouse_pathology.ontology
def: "Neoplasms derived from the non-germ cell derived tissues of the testis and ovary." [Pathbase: Curation]
is_a: MPATH:309 ! gonadal tumor

[Term]
id: MPATH:328
name: leydig cell tumor
namespace: mouse_pathology.ontology
def: "Tumor derived from Leydig cells (M-8650/1)." [Mahler M; Sundberg JP ( 1997) Spontaneous Leydig cell tumors in inbred laboratory mice Lab Animal Science 47:148-52]
synonym: "Interstitial cell tumor, benign" RELATED [Pathbase: Curation]
synonym: "Leydig cell adenoma" RELATED [Pathbase: Curation]
is_a: MPATH:323 ! gonadal somatic cell tumor

[Term]
id: MPATH:33
name: intracellular and extracellular accumulation
namespace: mouse_pathology.ontology
def: "Accumulation of substances within, on the surface of or between cells." [Pathbase: Pathology Committee]
is_a: MPATH:1 ! cell and tissue damage

[Term]
id: MPATH:331
name: sertoli cell tumor
namespace: mouse_pathology.ontology
def: "Tumor derived from sex cord/stromal cells; Sertoli cells and can occur in both testis and ovary. (M-8640/1)." [Pathbase: Pathology Committee]
synonym: "Androblastoma" RELATED [Pathbase: Curation]
synonym: "arrhenoblastoma" RELATED [Pathbase: Curation]
synonym: "gonadal stromal tumor" RELATED [Pathbase: Curation]
synonym: "sex cord stromal tumor" RELATED [Pathbase: Curation]
synonym: "sustentacluar tumor" RELATED [Pathbase: Curation]
is_a: MPATH:323 ! gonadal somatic cell tumor

[Term]
id: MPATH:335
name: hematopoietic/lymphoid malignancies/disorder
namespace: mouse_pathology.ontology
def: "Proliferative disorders and malignancies of the lymphoid and non lymphoid haematopoietic lineages." [URL:http\://www.bloodjournal.org/cgi/content/full/100/1/238/DC1/2]
is_a: MPATH:218 ! neoplasm

[Term]
id: MPATH:34
name: amyloid deposition
namespace: mouse_pathology.ontology
def: "Extracellular deposition of amyloid protein." [ISBN:0781727286]
comment: Any group of chemically diverse proteins that appears microscopically homogeneous, but is composed of linear non-branching aggregated fibrils aranged in sheets when see under the electron microscope.
synonym: "Amyloidosis" RELATED [Pathbase: Curation]
is_a: MPATH:33 ! intracellular and extracellular accumulation

[Term]
id: MPATH:342
name: myeloid leukaemia
namespace: mouse_pathology.ontology
def: "Leukaemias of the myeloid lineage." [PMID:12070033]
synonym: "granulocytic leukaemia" RELATED [Pathbase: Curation]
xref: URL:http\://www.bloodjournal.org/cgi/content/full/100/1/238/DC1/2
is_a: MPATH:496 ! Non-Lymphoid leukaemias

[Term]
id: MPATH:346
name: autoimmune mediated disease
namespace: mouse_pathology.ontology
is_a: MPATH:194 ! immune mediated disease
created_by: George Gkoutos
creation_date: 2011-03-22T01:12:01Z

[Term]
id: MPATH:351
name: thymoma
namespace: mouse_pathology.ontology
def: "A neoplasm in the anterior mediastinum, originating from thymic tissue, usually benign, and frequently encapsulated; occasionally invasive, but metastases are rare; histologically, consists of any type of thymic epithelial cell as well as lymphocytes that are usually abundant. (M-8580/1)." [ISBN:0781727286]
is_a: MPATH:556 ! potentially cancerous lesions

[Term]
id: MPATH:352
name: hepatic tumor
namespace: mouse_pathology.ontology
def: "Tumors of the liver and biliary apparatus." [Pathbase: Curation]
is_a: MPATH:218 ! neoplasm

[Term]
id: MPATH:353
name: hepatocellular adenoma
namespace: mouse_pathology.ontology
def: "Benign neoplasm derived from hepatocytes. (M- 8170/0)." [Pathbase: Curation]
synonym: "hepatic adenoma, benign, liver cell tumor, benign" RELATED [Pathbase: Curation]
synonym: "hepatoma, benign" RELATED [Pathbase: Curation]
synonym: "nodule type A" RELATED [Pathbase: Curation]
is_a: MPATH:270 ! adenoma
is_a: MPATH:352 ! hepatic tumor

[Term]
id: MPATH:354
name: cholangiocarcinoma
namespace: mouse_pathology.ontology
def: "Malignant tumor derived from the bile duct epithelium. (M8160/3)." [Pathbase: Pathology Committee]
is_a: MPATH:352 ! hepatic tumor
is_a: MPATH:549 ! carcinoma

[Term]
id: MPATH:356
name: hepatoblastoma
namespace: mouse_pathology.ontology
def: "Malignant neoplasm of the liver of unknown origin . Liver blastemal cells, neoplastic hepatocytes, oval cells and biliary epithelial cells have been proposed. (M- 8970/3)." [Pathbase: Curation]
synonym: "embryonal hepatoma" RELATED [Pathbase: Curation]
synonym: "tumor, mixed, poorly differentiated" RELATED [Pathbase: Curation]
is_a: MPATH:352 ! hepatic tumor

[Term]
id: MPATH:357
name: hepatocellular carcinoma
namespace: mouse_pathology.ontology
def: "Malignant tumor derived from hepatocytes. (M- 8170/3)." [Book: Bannasche; P and Zerban; H. Preneoplastic and neoplastic lesions of the rat iver. In; Pathology of neoplasia and preneoplasia in rodents; P. Bannasch and W. Goessner; Editors. 1997. Schattauer; Stuttgart. p. 18-63]
synonym: "carcinoma, trabecular" RELATED [Pathbase: Curation]
synonym: "carcinoma, trabecular (liver)" RELATED [Pathbase: Curation]
synonym: "hepatoma, malignant" RELATED [Pathbase: Curation]
synonym: "nodule type B" RELATED [Pathbase: Curation]
is_a: MPATH:352 ! hepatic tumor
is_a: MPATH:549 ! carcinoma

[Term]
id: MPATH:358
name: melanocytic tumor
namespace: mouse_pathology.ontology
def: "Tumors derived from melanocytes." [Pathbase: Pathology Committee]
is_a: MPATH:219 ! adnexal and skin appendage tumor

[Term]
id: MPATH:359
name: melanoma
namespace: mouse_pathology.ontology
def: "Tumor of neurectodermal origin, usually melanocytes, showing dense deposition of melanin granules, although amelanotic melanomas have been reported. (M-8720/3)." [Book: Klein-Szanto; A.J.; Neoplastic and preneoplastic lesions of the mouse skin; in Pathology of neoplasia and preneoplasia in rodents; P. Bannasch and W. Goessner; Editors. 1997. Schattauer; Stuttgart. p. 1-18]
synonym: "melanosarcoma" RELATED [Pathbase: Curation]
synonym: "melanosarcoma, malignant melanoma" RELATED [Pathbase: Curation]
xref: URL: http\://emice.nci.nih.gov/emice/mouse_models/organ_models/skin_models/malignant_melanoma#melanoma_table
is_a: MPATH:358 ! melanocytic tumor

[Term]
id: MPATH:36
name: calcium deposition
namespace: mouse_pathology.ontology
def: "Intra or extracellular deposition of calcium usually as calcium phosphate." [Pathbase: Curation]
is_a: MPATH:555 ! mineralisation

[Term]
id: MPATH:360
name: melanoma in situ
namespace: mouse_pathology.ontology
def: "A potentially malignant lesion, melanoma in situ is the first phase of growth of melanoma, in which it is still confined to the epithelial domain (epidermis and adnexa) and has not passed through the basement membrane. (M-8720/2)." [Pathbase: Pathology Committee]
synonym: "level I melanoma" RELATED [Pathbase: Curation]
is_a: MPATH:358 ! melanocytic tumor
is_a: MPATH:556 ! potentially cancerous lesions

[Term]
id: MPATH:361
name: naevus
namespace: mouse_pathology.ontology
def: "Local lesion of the skin, often colored by hyperpigmentation or increased vascularity. May be predominantly epidermal, adnexal, melanocytic, vascular, or mesodermal, or a compound overgrowth of these tissues. Not necessarily pre-malignant. (M-8720/0)." [Pathbase: Pathology Committee]
synonym: "mole (sensu melanocytic nevus)" RELATED [Pathbase: Curation]
is_a: MPATH:358 ! melanocytic tumor

[Term]
id: MPATH:365
name: mesothelioma
namespace: mouse_pathology.ontology
def: "Benign or malignant neoplasm derived from the lining cells of the pleura and peritoneum, composed of spindle cells or fibrous tissue which may enclose glandlike spaces lined by cuboidal cells. Epithelioid, fibrous, cystis, papillary, and sarcomatoid variants. (M- 9050/3)." [Pathbase: Curation]
is_a: MPATH:218 ! neoplasm

[Term]
id: MPATH:366
name: neuroendocrine tumor
namespace: mouse_pathology.ontology
def: "Neoplasms derived from the neuroendocrine system." [Pathbase: Curation]
is_a: MPATH:218 ! neoplasm

[Term]
id: MPATH:370
name: primitive neurectodermal tumor
namespace: mouse_pathology.ontology
def: "Primitive neuroectodermal tumors (PNET) are neoplasms derived from primitive neural stem cells either in the CNS or the periphery . These are small-cell, malignant embryonal tumors showing divergent differentiation of variable degree along neuronal, glial, or rarely mesenchymal lines. (M-9473/3, M-9364/3)." [ISBN-13:9783794515530]
synonym: "PNET" RELATED [Pathbase: Curation]
is_a: MPATH:373 ! CNS progenitor tumor
is_a: MPATH:570 ! peripheral nervous system tumors

[Term]
id: MPATH:371
name: small cell carcinoma
namespace: mouse_pathology.ontology
def: "Neuroendocrine cell derived anaplastic carcinoma composed of small cells, usually of the lung producing a variety of peptide hormones. (M-8041/3). 1.2.3.4 of MMHCC classification." [PMID:15059877]
comment: see: Meuwissen, R., Linn, S.C., Linnoila, R.I. et al. (2003) Induction of small cell lung cancer by somatic inactivation of both Trp53 and Rb1 in a conditional mouse model. Cancer cell, 4: 181-189. AND Calbo, J., Meuwissen, R., van Montfort, E. et al. (2005) Genotype-phenotype relationships in a mouse model for human small-cell lung cancer. Cold Spring Harbor symposia on quantitative biology, 70: 225-232. AND Meuwissen, R. and Berns, A. (2005) Mouse models for human lung cancer. Genes & development, 19: 643-664.
synonym: "oat cell carcinoma" RELATED [Pathbase: Curation]
xref: URL: http\://emice.nci.nih.gov/mouse_models/organ_models/lung_models/murinecancer/tumorclass
is_a: MPATH:366 ! neuroendocrine tumor
is_a: MPATH:549 ! carcinoma

[Term]
id: MPATH:373
name: CNS progenitor tumor
namespace: mouse_pathology.ontology
def: "Neoplasms derived from neuroepithelial precursors." [Pathbase: Pathology Committee]
comment: Renamed from neuroepitheliomatous tumor, to reflect primitive origins of this class of tumor.
is_a: MPATH:565 ! tumors of neurepithelial tissue

[Term]
id: MPATH:375
name: ganglioneuroma
namespace: mouse_pathology.ontology
def: "A benign neoplasm composed of mature ganglionic neurons scattered singly or in clumps within a relatively abundant and dense stroma of neurofibrils and collagenous fibers. (M-9490/0)." [Pathbase: Pathology Committee]
is_a: MPATH:570 ! peripheral nervous system tumors

[Term]
id: MPATH:376
name: neuroblastoma
namespace: mouse_pathology.ontology
def: "A malignant neoplasm characterized by immature, poorly differentiated nerve cells of embryonic type. (M-9500/3)." [ISBN-13:9783794515530]
is_a: MPATH:373 ! CNS progenitor tumor

[Term]
id: MPATH:377
name: pheochromocytoma
namespace: mouse_pathology.ontology
def: "A catecholamine-secreting tumor arising from the chromaffin cells of the sympathetic nervous system or adrenal medulla. May be benign or malignant. [See MPATH 398]. (M- 8510/3)." [Pathbase: Pathology Committee]
is_a: MPATH:366 ! neuroendocrine tumor

[Term]
id: MPATH:378
name: retinoblastoma
namespace: mouse_pathology.ontology
def: "Malignant juvenile neoplasm of the eye derived from primitive retinal precursor cells. (M- 9510/3)." [Pathbase: Curation]
is_a: MPATH:373 ! CNS progenitor tumor

[Term]
id: MPATH:379
name: odontogenic tumor
namespace: mouse_pathology.ontology
def: "Neoplasm arising from the tissues of the odontogenic apparatus. These tumors are derived from ectodermal tissue (epithelial tumors) or from mesodermal tissue (connective tissue tumors) or are composed of both components (mixed or composite odontogenic tumors) ." [Pathbase: Pathology Committee]
is_a: MPATH:218 ! neoplasm

[Term]
id: MPATH:387
name: odontoma
namespace: mouse_pathology.ontology
def: "Hamartomatous malformation of odontogenic tissue. It may vary from nondescript masses of dental tissue (complex odontoma) to multiple well-formed teeth (compound odontoma). Cf ameloblastic fibro-odontoma. (M-9280/0)." [ISBN:0781727286]
is_a: MPATH:254 ! complex tumor
is_a: MPATH:379 ! odontogenic tumor
is_a: MPATH:74 ! hamartoma

[Term]
id: MPATH:388
name: osseous and chondromatous tumor
namespace: mouse_pathology.ontology
def: "Neoplasms of bone and cartilage." [Pathbase: Curation]
is_a: MPATH:218 ! neoplasm

[Term]
id: MPATH:392
name: chondrosarcoma
namespace: mouse_pathology.ontology
def: "Malignant neoplasm derived form pluripotential mesenchymal cells, chondrocytes or chondroblasts. No production of osteoid. (M-9220/3)." [Pathbase: Pathology Committee]
is_a: MPATH:388 ! osseous and chondromatous tumor

[Term]
id: MPATH:396
name: osteoma
namespace: mouse_pathology.ontology
def: "Benign neoplasm derived from osteoblasts or osteocytes composed of very dense bone with predominantly woven structure. ( M-9180/0)." [Book: Luz; A and Gessner; W. ; Neoplastic bone lesions of the mouse; in Pathology of neoplasia and preneoplasia in rodents; P. Bannasch and W. Goessner; Editors. 1997. Schattauer; Stuttgart. p. 142-154]
synonym: "cancellous osteoma" RELATED [Pathbase: Curation]
synonym: "compact osteoma" RELATED [Pathbase: Curation]
synonym: "juxtacortical osteoma" RELATED [Pathbase: Curation]
synonym: "medullary osteoma" RELATED [Pathbase: Curation]
synonym: "osteoid osteoma" RELATED [Pathbase: Curation]
synonym: "spongious osteoma" RELATED [Pathbase: Curation]
synonym: "trabecular osteoma" RELATED [Pathbase: Curation]
is_a: MPATH:388 ! osseous and chondromatous tumor

[Term]
id: MPATH:397
name: osteosarcoma
namespace: mouse_pathology.ontology
def: "Malignant neoplasm derived form mesenchymal stem cells, osteoblasts or osteocytes. Highly invasive and destructive tumor rising in the skeleton with osteoid and immature woven bone. (M-9180/3)." [Pathbase: Curation]
synonym: "osteogenic sarcoma" RELATED [Pathbase: Curation]
is_a: MPATH:388 ! osseous and chondromatous tumor

[Term]
id: MPATH:398
name: paragangliomas and glomus tumor
namespace: mouse_pathology.ontology
def: "Generally benign neoplasms of CHIEF cells arising from neuroectodermal tissues, found in various parts of the body. Note that until recently, glomus tumors were believed to be derived from specialised vascular cells, which is incorrect. Paraganglioma is the preferred term.The nomenclature for pheochromocytoma and paraganglioma is inconsistent. The term paraganglioma is used to refer to any extra-adrenal tumor of the paraganglion system or nonfunctional tumor of the paraganglion system. Functional tumors are referred extra-adrenal pheochromocytoma." [Pathbase: Curation]
is_a: MPATH:366 ! neuroendocrine tumor

[Term]
id: MPATH:4
name: necrosis
namespace: mouse_pathology.ontology
def: "Morpholological changes after intravital (Pathologic) death of one or more cells, or of a portion of tissue or organ, resulting from irreversible damage;characterised by mitochondrial swelling, nuclear pyknosis, karyolysis, swollen and abnormally pale basophilic staining; or karyorrhexis, rupture and fragmentation of the nucleus. Energy independent cf. Apoptosis MPATH 3." [ISBN:0781727286]
is_a: MPATH:2 ! cell death

[Term]
id: MPATH:403
name: paraganglioma
namespace: mouse_pathology.ontology
def: "A neoplasm composed of derivatives of CHIEF cells usually in single encapsulated nodular masses surrounded with sustentacular cells. ( M- 8711/0)." [Pathbase: Curation]
synonym: "chemodectomas" RELATED [Pathbase: Curation]
synonym: "glomus tumor" RELATED [Pathbase: Curation]
synonym: "non-chromaffin paragangliomas" RELATED [Pathbase: Curation]
is_a: MPATH:398 ! paragangliomas and glomus tumor

[Term]
id: MPATH:404
name: soft tissue tumor
namespace: mouse_pathology.ontology
def: "Neoplasms of the soft and connective tissues." [Pathbase: Curation]
is_a: MPATH:218 ! neoplasm

[Term]
id: MPATH:405
name: chordoma
namespace: mouse_pathology.ontology
def: "Believed to arise from primitive notochord remnants . Usually occurs along the axial skeleton and is characterised by the presence of bubble cells containing large unstained cytoplasmic vacuoles with central or eccentricc nuclei. Benign but locally invasive. (M-9370/3)." [Pathbase: Curation]
is_a: MPATH:404 ! soft tissue tumor

[Term]
id: MPATH:407
name: fibroma
namespace: mouse_pathology.ontology
def: "Benign neoplasm of fibroblasts/fibrocytes with poor/moderate cellularity. (M-8810/0)." [Pathbase: Pathology Committee]
comment: "Soft tissue" qualifier removed by Pathology Panel to increase scope of term.
is_a: MPATH:404 ! soft tissue tumor
is_a: MPATH:551 ! sarcoma

[Term]
id: MPATH:408
name: soft tissue fibrosarcoma
namespace: mouse_pathology.ontology
def: "Malignant tumor derived from pluripotential mesenchymal stem cells; fibroblasts, fibrocytes (M-8810/3)." [Pathbase: Pathology Committee]
synonym: "fibrosarcoma" EXACT []
is_a: MPATH:404 ! soft tissue tumor
is_a: MPATH:551 ! sarcoma

[Term]
id: MPATH:415
name: lipomatous tumor
namespace: mouse_pathology.ontology
def: "Tumors derived from the lipogenic lineage or showing predominantly lipomatous differentiation." [Pathbase: Curation]
is_a: MPATH:404 ! soft tissue tumor

[Term]
id: MPATH:416
name: angiomyolipoma
namespace: mouse_pathology.ontology
def: "Benign renal neoplasm composed of fat, vascular, and smooth muscle elements. Associated with tuberous sclerosis in humans. Aetiology unknown, but the combination of elements may reflect a lesion specific pattern of metaplasia. (M-8860/0)." [Pathbase: Pathology Committee]
is_a: MPATH:254 ! complex tumor
is_a: MPATH:415 ! lipomatous tumor

[Term]
id: MPATH:417
name: lipoma
namespace: mouse_pathology.ontology
def: "Benign neoplasia derived from lipoblasts or lipocytes of white or brown fat. May be angiomatous or hibernomatous. (M- 8850/0)." [Pathbase: Pathology Committee]
is_a: MPATH:415 ! lipomatous tumor

[Term]
id: MPATH:419
name: lymphatic vessel tumor
namespace: mouse_pathology.ontology
def: "Neoplasms of the lymphatic vessels." [Pathbase: Curation]
is_a: MPATH:404 ! soft tissue tumor

[Term]
id: MPATH:420
name: lymphangioma
namespace: mouse_pathology.ontology
def: "Benign hamartomatous malformation of the lymphatic ducts. Usually found in the skin and may be superficial or deep. (M-9170/0)." [ISBN:0781727286]
synonym: "Hygroma" BROAD [ISBN:0-19-261976-4]
is_a: MPATH:419 ! lymphatic vessel tumor
is_a: MPATH:74 ! hamartoma

[Term]
id: MPATH:423
name: myomatous tumor
namespace: mouse_pathology.ontology
def: "Neoplasms derived from myogenic lineages or predominantly composed of cells showing myomatous differentiation." [Pathbase: Curation]
is_a: MPATH:404 ! soft tissue tumor

[Term]
id: MPATH:425
name: leiomyoma
namespace: mouse_pathology.ontology
def: "Benign neoplasm derived from smooth muscle cells. (M-8890/0)." [Pathbase: Curation]
is_a: MPATH:423 ! myomatous tumor

[Term]
id: MPATH:426
name: leiomyosarcoma
namespace: mouse_pathology.ontology
def: "Malignant tumor derived form pluripotential mesenchymal stem cells or smooth muscle cells. (M- 8890/3)." [Pathbase: Curation]
is_a: MPATH:423 ! myomatous tumor
is_a: MPATH:551 ! sarcoma

[Term]
id: MPATH:428
name: rhabdomyosarcoma
namespace: mouse_pathology.ontology
def: "Malignant tumor of striated muscle or pluripotential mesenchymal stem cells. (M-8900/3)." [Pathbase: Curation]
is_a: MPATH:423 ! myomatous tumor
is_a: MPATH:551 ! sarcoma

[Term]
id: MPATH:429
name: myxomatous tumor
namespace: mouse_pathology.ontology
def: "Neoplasms resembling primitive mesenchymal tissue with a soft mucous matrix." [Pathbase: Curation]
is_a: MPATH:404 ! soft tissue tumor

[Term]
id: MPATH:431
name: myxoma
namespace: mouse_pathology.ontology
def: "A benign neoplasm derived from pluripotential mesenchymal stem cells of connective tissue, consisting chiefly of polyhedral and stellate cells that are loosely embedded in a soft mucoid matrix. May show multiple differentiated components. (M-8840/0)." [Pathbase: Pathology Committee]
is_a: MPATH:429 ! myxomatous tumor

[Term]
id: MPATH:433
name: nerve sheath tumor
namespace: mouse_pathology.ontology
def: "Neoplasms of the nerve sheath." [Pathbase: Pathology Committee]
is_a: MPATH:404 ! soft tissue tumor
is_a: MPATH:570 ! peripheral nervous system tumors

[Term]
id: MPATH:435
name: neurofibroma
namespace: mouse_pathology.ontology
def: "Peripheral nerve tumor consisting of chaotic arrays of wavy schwann cell bundles and fibroblasts interspersed within a matrix rich in collagen and mucopolysaccharide. (M9540/0)." [ISBN-13:9783794515530]
is_a: MPATH:433 ! nerve sheath tumor

[Term]
id: MPATH:437
name: neurofibrosarcoma
namespace: mouse_pathology.ontology
def: "Malignant neoplasm derived from Schwann cells. (M-9540/3)." [ISBN-13:9783794515530]
synonym: "malignant peripheral nerve sheath tumor" RELATED [Pathbase: Curation]
is_a: MPATH:433 ! nerve sheath tumor
is_a: MPATH:551 ! sarcoma

[Term]
id: MPATH:438
name: schwannoma
namespace: mouse_pathology.ontology
def: "May be malignant or benign, Schwann cell derived tumor considered to be neurectodermal with some acquired mesenchymal features. (M-9560/0)." [ISBN-13:9783794515530]
synonym: "neurilemoma" RELATED [Pathbase: Curation]
synonym: "neurinoma, benign" RELATED [Pathbase: Curation]
is_a: MPATH:433 ! nerve sheath tumor

[Term]
id: MPATH:442
name: squamous cell tumor
namespace: mouse_pathology.ontology
def: "Neoplasms of stratified squamous epithelial cells." [Pathbase: Pathology Committee]
is_a: MPATH:218 ! neoplasm

[Term]
id: MPATH:445
name: papilloma
namespace: mouse_pathology.ontology
def: "A benign tumor consisting of villous or arborescent outgrowths of fibrovascular stroma covered by neoplastic epithelial cells (M-8050/0)." [Pathbase: Pathology Committee]
is_a: MPATH:264 ! fibroepithelial tumor
is_a: MPATH:556 ! potentially cancerous lesions

[Term]
id: MPATH:446
name: squamous cell carcinoma
namespace: mouse_pathology.ontology
def: "Malignant tumor derived from stratified squamous cells. (M-8070/3)." [Pathbase: Pathology Committee]
synonym: "carcinoma, epidermoid ( sensu epidermal derived tumors)" RELATED [Pathbase: Curation]
is_a: MPATH:219 ! adnexal and skin appendage tumor
is_a: MPATH:442 ! squamous cell tumor
is_a: MPATH:549 ! carcinoma

[Term]
id: MPATH:450
name: transitional cell tumor
namespace: mouse_pathology.ontology
def: "Neoplasms of transitional epithelia, eg kidney, ureter , bladder , cervix." [Pathbase: Pathology Committee]
is_a: MPATH:218 ! neoplasm

[Term]
id: MPATH:451
name: transitional cell carcinoma
namespace: mouse_pathology.ontology
def: "Malignant neoplasm of transitional cells (M-8120/3)." [Pathbase: Curation]
is_a: MPATH:450 ! transitional cell tumor
is_a: MPATH:549 ! carcinoma

[Term]
id: MPATH:474
name: ectasia
namespace: mouse_pathology.ontology
def: "Dilation of a tubular structure." [Pathbase: Pathology Committee]
comment: Often associated with an obstruction.
is_a: MPATH:66 ! dilatation

[Term]
id: MPATH:476
name: telangiectasia
namespace: mouse_pathology.ontology
def: "A lesion formed by a dilated capillary or terminal artery." [Pathbase: Curation]
is_a: MPATH:474 ! ectasia

[Term]
id: MPATH:490
name: adenomatous polyp
namespace: mouse_pathology.ontology
def: "Benign neoplastic growth containing areas of adenomatous structure (progression)." [Pathbase: Curation]
synonym: "polypoid adenoma, cellular polyp." RELATED [Pathbase: Curation]
is_a: MPATH:270 ! adenoma
relationship: part_of MPATH:271 ! adenomatous polyposis coli

[Term]
id: MPATH:496
name: Non-Lymphoid leukaemias
namespace: mouse_pathology.ontology
def: "Neoplasms of non-lymphoid haematopoietic lineage. Must have at least 20% blast cells to meet this definition." [PMID:12070033]
xref: URL:http\://www.bloodjournal.org/cgi/content/full/100/1/238/DC1/2
is_a: MPATH:515 ! Non-Lymphoid neoplasias

[Term]
id: MPATH:502
name: monocytic leukaemia
namespace: mouse_pathology.ontology
def: "Leukaemia in which neoplastic cells are poorly or moderately differentiated with a monocytic but no neutrophilic component. At least 20% of the cells must be blasts." [PMID:12070033]
xref: URL:http\://www.bloodjournal.org/cgi/content/full/100/1/238/DC1/2
is_a: MPATH:342 ! myeloid leukaemia

[Term]
id: MPATH:504
name: non-lymphoid hematopoietic sarcomas
namespace: mouse_pathology.ontology
def: "Solid tumor mass composed of non-lymphoid haematopoietic cells." [PMID:12070033]
xref: URL:http\://www.bloodjournal.org/cgi/content/full/100/1/238/DC1/2
is_a: MPATH:335 ! hematopoietic/lymphoid malignancies/disorder
is_a: MPATH:551 ! sarcoma

[Term]
id: MPATH:506
name: histiocytic sarcoma
namespace: mouse_pathology.ontology
def: "Solid tumor mass composed predominantly of histiocytic cells (M-9775/3)." [PMID:12070033]
synonym: "histiocytic lymphoma" RELATED [Pathbase: Curation]
synonym: "Kupffer cell sarcoma (sensu liver)" RELATED [Pathbase: Curation]
synonym: "malignant lymphoma, histiocytic type" RELATED [Pathbase: Curation]
synonym: "reticulum cell sarcoma, type A" RELATED [Pathbase: Curation]
synonym: "reticulum cell sarcoma, type A, reticulosarcoma" RELATED [Pathbase: Curation]
xref: URL:http\://www.bloodjournal.org/cgi/content/full/100/1/238/DC1/2
is_a: MPATH:504 ! non-lymphoid hematopoietic sarcomas

[Term]
id: MPATH:513
name: Lymphoid neoplasms
namespace: mouse_pathology.ontology
def: "Neoplasms of the B or T cell lineage." [PMID:12070034]
is_a: MPATH:335 ! hematopoietic/lymphoid malignancies/disorder

[Term]
id: MPATH:515
name: Non-Lymphoid neoplasias
namespace: mouse_pathology.ontology
def: "Hematological neoplasias of non-lymphoid origin." [PMID:12070033]
xref: URL:http\://www.bloodjournal.org/cgi/content/full/100/1/238/DC1/2
is_a: MPATH:335 ! hematopoietic/lymphoid malignancies/disorder

[Term]
id: MPATH:516
name: B-cell neoplasms
namespace: mouse_pathology.ontology
def: "Neoplasm of the B cell lymphoid lineage." [Pathbase: Curation]
is_a: MPATH:513 ! Lymphoid neoplasms

[Term]
id: MPATH:519
name: Mature B-cell neoplasms
namespace: mouse_pathology.ontology
def: "Lymphomas originating in peripheral B cells." [PMID:12070034]
is_a: MPATH:516 ! B-cell neoplasms

[Term]
id: MPATH:530
name: Plasma cell neoplasms
namespace: mouse_pathology.ontology
def: "Diffuse proliferation of mature plasma cells. Clonal by definition. Includes the equivalent of human myeloma (ICD-O 9732/3)." [PMID:12070034]
synonym: "Myeloma ( human )" RELATED [Pathbase: Curation]
xref: URL: http\://emice.nci.nih.gov/emice/mouse_models/organ_models/hema_models/hema_mouse_class
is_a: MPATH:516 ! B-cell neoplasms

[Term]
id: MPATH:532
name: plasmacytoma
namespace: mouse_pathology.ontology
def: "Diffuse proliferation of mature plasma cells. Clonal by definition." [PMID:12070034]
comment: Tissue, usually lymph nodes, that contain unusually large numbers of normal appearing plasma cells. While these may be plasmacytomas, additional work is needed to confirm this latter diagnosis.
xref: URL: http\://emice.nci.nih.gov/emice/mouse_models/organ_models/hema_models/hema_mouse_class
is_a: MPATH:530 ! Plasma cell neoplasms

[Term]
id: MPATH:535
name: T-cell neoplasms
namespace: mouse_pathology.ontology
def: "Neoplasms derived from cells of the T lymphocyte lineage." [PMID:12070034]
is_a: MPATH:513 ! Lymphoid neoplasms

[Term]
id: MPATH:536
name: precursor T-cell neoplasms
namespace: mouse_pathology.ontology
def: "Neoplasms of precursor T cells." [PMID:12070034]
is_a: MPATH:535 ! T-cell neoplasms

[Term]
id: MPATH:537
name: precursor T-cell lymphoblastic lymphoma/leukaemia
namespace: mouse_pathology.ontology
def: "Precursor T cell derived neoplasia. Most commonly found in the thymus." [PMID:12070034]
synonym: "thymic lymphoma" RELATED [Pathbase: Curation]
is_a: MPATH:536 ! precursor T-cell neoplasms

[Term]
id: MPATH:549
name: carcinoma
namespace: mouse_pathology.ontology
def: "Any of various types of malignant neoplasm derived from epithelial cells, chiefly glandular (adenocarcinoma) or squamous (squamous cell carcinoma)." [Pathbase: Curation]
is_a: MPATH:218 ! neoplasm

[Term]
id: MPATH:55
name: developmental and structural abnormality
namespace: mouse_pathology.ontology
def: "Developmental and structural abnormalities occurring during embryonic development or during adult life." [Pathbase: Pathology Committee]
is_a: MPATH:603 ! pathological anatomical entity

[Term]
id: MPATH:551
name: sarcoma
namespace: mouse_pathology.ontology
def: "A connective tissue neoplasm, usually highly malignant, formed by proliferation of mesodermal cells." [Pathbase: Curation]
is_a: MPATH:218 ! neoplasm

[Term]
id: MPATH:555
name: mineralisation
namespace: mouse_pathology.ontology
def: "Deposition of any homogeneous inorganic material." [ISBN:0781727286]
is_a: MPATH:33 ! intracellular and extracellular accumulation

[Term]
id: MPATH:556
name: potentially cancerous lesions
namespace: mouse_pathology.ontology
def: "Lesions which in some cases have the potential to become progressively growing malignant tumors." [Pathbase: Pathology Committee]
is_a: MPATH:218 ! neoplasm

[Term]
id: MPATH:56
name: developmental or adult structural  defect
namespace: mouse_pathology.ontology
def: "Structural, physical or other general defect of prenatal development of the embryo and the placenta, or such as are acquired in the adult." [Pathbase: Pathology Committee]
is_a: MPATH:55 ! developmental and structural abnormality

[Term]
id: MPATH:564
name: glioblastoma
namespace: mouse_pathology.ontology
def: "Develop primarily through increasing anaplasia of well differentiated gliomas, mainly astrocytomas or oligodendrogliomas. Typically large and contain cells of different sizes with irrregular nuclei and atypical mitotic figures. (M-9440/3)." [ISBN-13:9783794515530]
comment: Also see Weiss, W.W, Israel, M. Cobbs, C., et al. (2002) Oncogene 21, 7453-7463.
synonym: "glioblastoma multiforme" RELATED [Pathbase: Curation]
synonym: "monstrocytoma" RELATED [Pathbase: Curation]
is_a: MPATH:249 ! glioma

[Term]
id: MPATH:565
name: tumors of neurepithelial tissue
namespace: mouse_pathology.ontology
def: "Tumors of neuronal and non-neuronal cells derived from embryonic neurepithelium." [Pathbase: Pathology Committee]
is_a: MPATH:243 ! central nervous system tumor

[Term]
id: MPATH:566
name: tumors of the meninges
namespace: mouse_pathology.ontology
def: "tumors of the meninges" [Pathbase: Curation]
is_a: MPATH:243 ! central nervous system tumor

[Term]
id: MPATH:570
name: peripheral nervous system tumors
namespace: mouse_pathology.ontology
def: "Tumors of the peripheral nervous system." [Pathbase: Pathology Committee]
is_a: MPATH:218 ! neoplasm

[Term]
id: MPATH:571
name: pilomatricoma
namespace: mouse_pathology.ontology
def: "Tumor composed of the epithelial components of the most proximal (trichogenic) portion of the hair follicle associated with an aberrent hair cortex type of cornification (ghost cells or shadow cells). The most primitive cellular component consists of basophilic cells having scanty cytoplasm and nuclei that occasionally overlap to some extent. In humans mineralisation is common." [See: Gat; U.; DasGupta; R.; Degenstein; L. and Fuchs; E. (1998) De Novo hair follicle morphogenesis and hair tumors in mice expressing a truncated beta-catenin in skin Cell; 95; 605-614.]
is_a: MPATH:575 ! basaloid follicular neoplasms

[Term]
id: MPATH:574
name: nephroblastomatosis
namespace: mouse_pathology.ontology
def: "Persistence of metanephrogenic blastema or its presence in the wrong place or at the wrong time. Associated with hyperplastic nephrogenic rests." [PMID:8383276]
is_a: MPATH:64 ! developmental dysplasia

[Term]
id: MPATH:575
name: basaloid follicular neoplasms
namespace: mouse_pathology.ontology
def: "This is a new diagnostic term that the MMHC pathology panel felt best described a diagnostically challenging set of tumors that share the feature of being compose of basaloid cells showing follicular differentiation to some extent. These tumors are common in GEM involving the hedgehog signaling pathway and frequently have more than one of the histologic patterns listed below. The designation of benign and malignant has been excluded from the primary diagnosis purposely, as this is frequently difficult to determine in these characteristically well circumscribed tumors. The presence of a disorganized (non-palisaded) sheet-like growth pattern, tumor necrosis, or numerous mitoses are felt to represent malignant transformation." [URL:http\://emice.nci.nih.gov/emice/mouse_models/organ_models/skin_models]
is_a: MPATH:219 ! adnexal and skin appendage tumor

[Term]
id: MPATH:576
name: trichofolliculoma
namespace: mouse_pathology.ontology
def: "Basaloid neoplasm with numerous mature hair follicles and hair formation." [URL:http\://emice.nci.nih.gov/emice/mouse_models/organ_models/skin_models]
relationship: part_of MPATH:575 ! basaloid follicular neoplasms

[Term]
id: MPATH:579
name: ulcer
namespace: mouse_pathology.ontology
def: "Loss of epithelium and the basement membrane (full thickness). Cf Erosion." [Pathbase: Pathology Committee]
is_a: MPATH:1 ! cell and tissue damage

[Term]
id: MPATH:596
name: pathological process
namespace: mouse_pathology.ontology
def: "The organic response of tissues to external insult, injury or underlying genetic or epigenetic lesion." [Pathbase: Pathology Committee]
is_a: MPATH:0 ! pathological entity

[Term]
id: MPATH:597
name: cell and tissue damage process
namespace: mouse_pathology.ontology
def: "Processes occurring during cell and tissue damage of either intrinsic or extrinsic etiology." [Pathbase: Pathology Committee]
is_a: MPATH:596 ! pathological process

[Term]
id: MPATH:599
name: developmental process abnormalities
namespace: mouse_pathology.ontology
def: "developmental process abnormalities" [Pathbase: Pathology Committee]
is_a: MPATH:596 ! pathological process

[Term]
id: MPATH:602
name: hyperplastic tissue
namespace: mouse_pathology.ontology
def: "An organ or a tissue with an abnormal increase in the number of cells as a consequence of cell proliferation." [Pathbase: Pathology Committee]
is_a: MPATH:126 ! growth and differentiation defect

[Term]
id: MPATH:603
name: pathological anatomical entity
namespace: mouse_pathology.ontology
def: "Anatomically located instance of pathological response or entity." [Pathbase: Pathology Committee]
is_a: MPATH:0 ! pathological entity

[Term]
id: MPATH:604
name: defective growth and differentiation process
namespace: mouse_pathology.ontology
def: "Abnormal increase or decrease in the rate of cell growth or cell division including associated changes in the differentiation state of adult cells." [Pathbase: Pathology Committee]
comment: Excludes abnormalities of developmental proliferation and differentiation.
is_a: MPATH:596 ! pathological process

[Term]
id: MPATH:605
name: metaplastic tissue
namespace: mouse_pathology.ontology
def: "A tissue or group of cells in which there has been abnormal transformation of an fully differentiated adult cell or tissue of one kind into a differentiated tissue of another kind." [Pathbase: Pathology Committee]
comment: Nearly exclusively used in an adult context.
is_a: MPATH:126 ! growth and differentiation defect

[Term]
id: MPATH:607
name: healing and repair structure
namespace: mouse_pathology.ontology
def: "Physical entity or structure associated with normal or abnormal tissue healing or repair following extrinsic or intrinsic damage." [Pathbase: Pathology Committee]
is_a: MPATH:603 ! pathological anatomical entity

[Term]
id: MPATH:608
name: abscess
namespace: mouse_pathology.ontology
def: "A circumscribed collection of purulent exudate frequently associated with swelling and other signs of inflammation." [ISBN:0781727286]
comment: Generally occur following damage or infection with subsequent inflammatory response. Result of the body`s defensive reaction to foreign material.
is_a: MPATH:607 ! healing and repair structure

[Term]
id: MPATH:615
name: cardiomyopathy
namespace: mouse_pathology.ontology
def: "A disease of the heart muscle or myocardium proper." [\:NCI Thesaurus / A7567983]
comment: Cardiomyopathies may be classified as either primary or secondary, on the basis of etiology, or on the pathophysiology of the lesion: hypertrophic, dilated, or restrictive.
is_a: MPATH:25 ! tissue specific degenerative process

[Term]
id: MPATH:62
name: cyst
namespace: mouse_pathology.ontology
def: "Formation of an epithelium bounded cavity not associated with neoplasia." [Pathbase: Pathology Committee]
is_a: MPATH:56 ! developmental or adult structural  defect

[Term]
id: MPATH:622
name: steatosis
namespace: mouse_pathology.ontology
def: "Abnormal retention of lipids within a cell. Physically apparent as lipid within liposomes of parenchymal cells." [Pathbase: Curation]
comment: Most commonly associated with degenerative change in the liver.
synonym: "adipose degeneration" RELATED [Pathbase: Curation]
synonym: "fatty change" RELATED [Pathbase: Curation]
synonym: "fatty degeneration" RELATED [Pathbase: Curation]
synonym: "lipidosis" EXACT []
is_a: MPATH:33 ! intracellular and extracellular accumulation

[Term]
id: MPATH:625
name: avulsion
namespace: mouse_pathology.ontology
def: "Tearing away or separation of two structures or parts." [ISBN:0781727286]
is_a: MPATH:56 ! developmental or adult structural  defect

[Term]
id: MPATH:629
name: cavernous hemangioma
namespace: mouse_pathology.ontology
def: "Deep cutaneous hemangioma with large dilated vascular spaces that manifests spontaneous involution." [ISBN:0781727286]
is_a: MPATH:240 ! hemangioma

[Term]
id: MPATH:64
name: developmental dysplasia
namespace: mouse_pathology.ontology
def: "Abnormal development (of organs or tissues) or an abnormal structure resulting from such growth." [Pathbase: Pathology Committee]
comment: The word dysplasia as commonly used refers to a precursor state to neoplasia. This is not the context used for this MPATH term.
is_a: MPATH:599 ! developmental process abnormalities

[Term]
id: MPATH:66
name: dilatation
namespace: mouse_pathology.ontology
def: "Increase in the diameter of an orifice or tubular structure beyond its normal dimensions." [Pathbase: Pathology Committee]
is_a: MPATH:56 ! developmental or adult structural  defect

[Term]
id: MPATH:675
name: psoriasiform dermatitis
namespace: mouse_pathology.ontology
is_a: MPATH:196 ! dermatitis
created_by: George Gkoutos
creation_date: 2011-02-19T04:09:12Z

[Term]
id: MPATH:68
name: diverticulum
namespace: mouse_pathology.ontology
def: "A blind ended outpouching through the wall of a tubular organ or bounded cavity." [Pathbase: Curation]
is_a: MPATH:56 ! developmental or adult structural  defect

[Term]
id: MPATH:695
name: spindle cell sarcoma
namespace: mouse_pathology.ontology
is_a: MPATH:551 ! sarcoma
created_by: George Gkoutos
creation_date: 2011-02-19T05:12:17Z

[Term]
id: MPATH:70
name: fistula
namespace: mouse_pathology.ontology
def: "An abnormal passage between two internal organs or leading from a cavity to the body surface." [Pathbase: Curation]
is_a: MPATH:56 ! developmental or adult structural  defect

[Term]
id: MPATH:707
name: angiolipoma
namespace: mouse_pathology.ontology
is_a: MPATH:415 ! lipomatous tumor
created_by: George Gkoutos
creation_date: 2011-02-20T08:44:41Z

[Term]
id: MPATH:709
name: alveolar rhabdomyosarcoma
namespace: mouse_pathology.ontology
def: "Malignant tumor of striated muscle or pluripotential mesenchymal stem cells composed mainly of small round cells, with some partial skeletal muscle differentiation." [ICD-O:8920/3]
is_a: MPATH:428 ! rhabdomyosarcoma
created_by: Paul
creation_date: 2011-06-06T03:24:13Z

[Term]
id: MPATH:710
name: embryonal rhabdomyosarcoma
namespace: mouse_pathology.ontology
def: "Malignant mesenchymal tumor that morphologically and phenotypically resembles embryonal skeletal muscle." [ICD-O:8910/3, ICDO-:8912/3]
comment: Includes spindle cell, botryoid, anaplastic.
synonym: " Rhabdopoietic Sarcoma" RELATED []
synonym: " Sarcoma Botryoides [Soft Tissues]" RELATED []
synonym: "Embryonal Sarcoma" RELATED []
synonym: "Malignant Rhabdomyoma" RELATED []
synonym: "Myosarcoma " EXACT []
is_a: MPATH:428 ! rhabdomyosarcoma
created_by: Paul
creation_date: 2011-06-06T03:31:11Z

[Term]
id: MPATH:718
name: pre-sacral teratoma
namespace: mouse_pathology.ontology
def: "Generally benign germ cell derived tumors of male or female containing derivatives from all three germ layers with differentiation in the malignant form being poor. Pre-sacral tumors located in the retrorectal space between the rectum and the sacrococcygeal part of the spine." [\:]
is_a: MPATH:322 ! teratoma
created_by: Paul
creation_date: 2011-06-06T03:39:01Z

[Term]
id: MPATH:722
name: rhabdomyoma
namespace: mouse_pathology.ontology
def: "Benign stromal tumors of the soft tissue with skeletal muscle differentiation." [ICD-O:M-8900/0, PMID:3525381]
comment: Adult and fetal types.
is_a: MPATH:423 ! myomatous tumor
created_by: Paul
creation_date: 2011-06-06T03:59:49Z

[Term]
id: MPATH:723
name: fibromatosis
namespace: mouse_pathology.ontology
def: "Systemic manifestation of MPATH: 407." [ICDO:M-8822/1]
synonym: " Musculoaponeurotic Fibromatosis" RELATED []
synonym: "Aggressive Fibromatosis" RELATED []
synonym: "Desmoid Tumor" EXACT []
synonym: "Plantar Fibromatosis (Ledderhose Disease)" RELATED []
is_a: MPATH:407 ! fibroma
created_by: Paul
creation_date: 2011-06-06T04:11:04Z

[Term]
id: MPATH:74
name: hamartoma
namespace: mouse_pathology.ontology
def: "A focal malformation resembling a neoplasm which results from faulty development of an organ; composed of an abnormal mixture of tissue elements, or an abnormal proportion of a single element. Growth and location are usually normal for that tissue cf. Heterotopia/Choristoma MPATH:76/MPATH:477." [ISBN:0781727286]
is_a: MPATH:56 ! developmental or adult structural  defect

[Term]
id: MPATH:81
name: perforation
namespace: mouse_pathology.ontology
def: "Presence of a hole/channel through a normally imperforate structure often a membrane or septum." [Pathbase: Pathology Committee]
is_a: MPATH:56 ! developmental or adult structural  defect

[Term]
id: MPATH:850
name: post-traumatic structural abnormality
namespace: mouse_pathology.ontology
def: "Morphological abnormality following trauma or related insult such as infection." [MPATH:curation]
is_a: MPATH:56 ! developmental or adult structural  defect
created_by: Paul
creation_date: 2012-03-24T03:28:03Z

[Term]
id: MPATH:851
name: auricular deformation
namespace: mouse_pathology.ontology
def: "acquired dysmorphology of the external pinna following trauma or infection." [MPATH:curation]
is_a: MPATH:850 ! post-traumatic structural abnormality
created_by: Paul
creation_date: 2012-03-24T03:29:48Z

[Term]
id: MPATH:86
name: organ specific developmental defect
namespace: mouse_pathology.ontology
def: "Developmental defect characteristic of a particular organ or organ system which may be a recognised syndrome or a complex defect showing multiple manifestations." [Pathbase: Curation]
is_a: MPATH:55 ! developmental and structural abnormality

[Term]
id: MPATH:89
name: cardiovascular developmental defect
namespace: mouse_pathology.ontology
def: "Abnormal development of the heart or vascular tissue resulting in morphological abnormality." [Pathbase: Curation]
is_a: MPATH:86 ! organ specific developmental defect

[Term]
id: MPATH:90
name: aneurysm
namespace: mouse_pathology.ontology
def: "Localised dilation of an artery or heart chamber usually due to an acquired or congenital weakness of the wall of the artery or chamber." [Pathbase: Pathology Committee]
is_a: MPATH:56 ! developmental or adult structural  defect

[Term]
id: MPATH:97
name: dissecting aneurysm
namespace: mouse_pathology.ontology
def: "Follows the presence of a hematoma in the wall of an artery Splitting of the media occurs, blood enters the split through a tear in the intima." [ISBN:0781727286]
is_a: MPATH:90 ! aneurysm

[Term]
id: MPATH:98
name: lymphangiectasis
namespace: mouse_pathology.ontology
def: "A stretching and widening of the lymphatic vessels." [Pathbase: Pathology Committee]
synonym: "Lymphectasia" RELATED [Pathbase: Curation]
synonym: "telangiectasia lymphatica" RELATED [Pathbase: Curation]
is_a: MPATH:474 ! ectasia
is_a: MPATH:89 ! cardiovascular developmental defect

[Typedef]
id: part_of
name: part of
namespace: mouse_pathology.ontology
is_transitive: true

